Complete termination proof

Regex/NFA/VM.lean
@@ -1,18 +1,52 @@
+import Regex.Lemmas
 import Regex.NFA.Basic
 
 -- TODO: use a bitvec?
 abbrev NodeSet (n : Nat) := { array : Array Bool // array.size = n }
 
+def NodeSet.empty {n : Nat} : NodeSet n :=
+  ⟨mkArray n false, by simp⟩
+
 def NodeSet.get (ns : NodeSet n) (i : Fin n) : Bool :=
-  ns.val.get (ns.property.symm ▸ i)
+  ns.val.get (i.cast ns.property.symm)
 
 def NodeSet.set (ns : NodeSet n) (i : Fin n) : NodeSet n :=
-  ⟨ns.val.set (ns.property.symm ▸ i) true, by simp [ns.property]⟩
+  ⟨ns.val.set (i.cast ns.property.symm) true, by simp [ns.property]⟩
+
+@[simp]
+theorem NodeSet.get_set_eq (ns : NodeSet n) (i : Fin n) :
+  (ns.set i).get i = true := by
+  simp [NodeSet.get, NodeSet.set]
+  rw [Array.get_set]
+  . simp
+  . simp [ns.property]
+
+theorem NodeSet.get_set_ne (ns : NodeSet n) (i j : Fin n) (ne : i.val ≠ j.val) :
+  (ns.set i).get j = ns.get j := by
+  simp [NodeSet.get, NodeSet.set]
+  rw [Array.get_set]
+  . simp [ne]
+  . simp [ns.property, ne]
 
 def NodeSet.unset (ns : NodeSet n) (i : Fin n) : NodeSet n :=
-  ⟨ns.val.set (ns.property.symm ▸ i) false, by simp [ns.property]⟩
+  ⟨ns.val.set (i.cast  ns.property.symm) false, by simp [ns.property]⟩
 
-def NodeSet.size (ns : NodeSet n) : Nat :=
+@[simp]
+theorem NodeSet.get_unset_eq (ns : NodeSet n) (i : Fin n) :
+  (ns.unset i).get i = false := by
+  simp [NodeSet.get, NodeSet.unset]
+  rw [Array.get_set]
+  . simp
+  . simp [ns.property]
+
+theorem NodeSet.get_unset_ne (ns : NodeSet n) (i j : Fin n) (ne : i.val ≠ j.val) :
+  (ns.unset i).get j = ns.get j := by
+  simp [NodeSet.get, NodeSet.unset]
+  rw [Array.get_set]
+  . simp [ne]
+  . simp [ns.property, ne]
+
+def NodeSet.count_set (ns : NodeSet n) : Nat :=
   go ns 0 0 (Nat.zero_le _)
 where
   go (ns : NodeSet n) (accum : Nat) (i : Nat) (hle : i ≤ n) : Nat :=
@@ -22,6 +56,83 @@ where
       have hlt : i < n := Nat.lt_of_le_of_ne hle h
       let accum := if ns.get ⟨i, hlt⟩ then accum + 1 else accum
       go ns accum (i + 1) hlt
+termination_by go _ => n - i
+
+def NodeSet.count_unset (ns : NodeSet n) : Nat :=
+  go ns 0 0 (Nat.zero_le _)
+where
+  go (ns : NodeSet n) (accum : Nat) (i : Nat) (hle : i ≤ n) : Nat :=
+    if h : i = n then
+      accum
+    else
+      have hlt : i < n := Nat.lt_of_le_of_ne hle h
+      let accum := if ns.get ⟨i, hlt⟩ then accum else accum + 1
+      go ns accum (i + 1) hlt
+termination_by go _ => n - i
+
+theorem NodeSet.lt_count_unset (ns : NodeSet n) (lt : x < n) (unset : ¬ ns.get ⟨x, lt⟩) :
+  (ns.set ⟨x, lt⟩).count_unset < ns.count_unset := by
+  let inv (i accum₁ accum₂ : Nat) : Prop :=
+    if i > x then
+      accum₁ + 1 = accum₂
+    else
+      accum₁ = accum₂
+
+  let rec go {i accum₁ accum₂ : Nat} (inv₀ : inv i accum₁ accum₂) (hle : i ≤ n) :
+    count_unset.go (ns.set ⟨x, lt⟩) accum₁ i hle + 1 = count_unset.go ns accum₂ i hle := by
+    simp [inv, lt] at *
+    split at inv₀
+    case inl lt' =>
+      unfold count_unset.go
+      cases Nat.decEq i n with
+      | isTrue eq =>
+        simp [eq]
+        exact inv₀
+      | isFalse neq =>
+        simp [neq]
+        have hlt : i < n := Nat.lt_of_le_of_ne hle neq
+        rw [NodeSet.get_set_ne]
+        . have lt'' : x < i + 1 := Nat.lt_trans lt' (Nat.lt_succ_self _)
+          have invt : inv (i + 1) accum₁ accum₂ := by
+            simp [inv, lt'', inv₀]
+          have invf : inv (i + 1) (accum₁ + 1) (accum₂ + 1) := by
+            simp [inv, lt'', inv₀]
+          cases ns.get ⟨i, hlt⟩ <;> simp
+          . exact go invf hlt
+          . exact go invt hlt
+        . simp
+          exact Nat.ne_of_lt lt'
+    case inr nlt' =>
+      have ge := Nat.ge_of_not_lt nlt'
+      cases Nat.lt_or_eq_of_le ge with
+      | inl gt =>
+        have hlt : i < n := Nat.lt_trans gt lt
+        have : i ≠ n := Nat.ne_of_lt hlt
+        unfold count_unset.go
+        simp [this]
+        rw [NodeSet.get_set_ne]
+        . have h : ¬ (i + 1 > x) := Nat.not_lt_of_ge gt
+          have invt : inv (i + 1) accum₁ accum₂ := by
+            simp [inv, h, inv₀]
+          have invf : inv (i + 1) (accum₁ + 1) (accum₂ + 1) := by
+            simp [inv, h, inv₀]
+          cases ns.get ⟨i, hlt⟩ <;> simp
+          . exact go invf hlt
+          . exact go invt hlt
+        . simp
+          exact Nat.ne_of_gt gt
+      | inr eq =>
+        simp [eq.symm] at unset
+        unfold count_unset.go
+        have : i ≠ n := Nat.ne_of_lt (eq ▸ lt)
+        simp [this, eq.symm, unset]
+        have inv : inv (i + 1) accum₁ (accum₂ + 1) := by
+          simp [inv, eq, inv₀]
+        exact eq ▸ (go inv (eq ▸ lt))
+
+  have inv₀ : inv 0 0 0 := by simp [inv, Nat.not_lt_zero x]
+  have := go inv₀ (Nat.zero_le _)
+  exact Nat.le_of_eq this
 termination_by go _ => n - i
 
 def NodeSet.clear (ns : NodeSet n) : NodeSet n :=
@@ -35,8 +146,71 @@ where
       go (ns.unset ⟨i, hlt⟩) (i + 1) hlt
 termination_by go _ => n - i
 
-def NodeSet.empty {n : Nat} : NodeSet n :=
-  ⟨mkArray n false, by simp⟩
+theorem NodeSet.get_empty {n : Nat} (i : Nat) (h : i < n) :
+  (NodeSet.empty : NodeSet n).get ⟨i, h⟩ = false := by
+  simp [empty, mkArray, NodeSet.get, Array.getElem_eq_data_get]
+
+theorem NodeSet.clear_eq_empty (ns : NodeSet n) : ns.clear = NodeSet.empty := by
+  have : ns.clear.val.size = n := ns.clear.property
+  apply Subtype.ext
+  apply Array.ext
+  . simp [this, empty]
+  . intro j h₁ h₂
+    have h : j < n := ns.clear.property ▸ h₁
+    have hc : ns.clear.get ⟨j, h⟩ = false := go ns 0 j (Nat.zero_le _) (Nat.zero_le _) h
+    simp [NodeSet.get] at hc
+    have he : empty.get ⟨j, h⟩ = false := NodeSet.get_empty j h
+    simp [NodeSet.get] at he
+    rw [hc, he]
+where
+  go (ns : NodeSet n) (i j : Nat) (hle : i ≤ n) (h₁ : i ≤ j) (h₂ : j < n) :
+    (NodeSet.clear.go ns i hle).get ⟨j, h₂⟩ = false := by
+    have h := go' ns i j hle h₂
+    simp [h₁] at h
+    exact h
+  go' (ns : NodeSet n) (i j : Nat) (hle : i ≤ n) (h : j < n) :
+    if i ≤ j then
+      (NodeSet.clear.go ns i hle).get ⟨j, h⟩ = false
+    else
+      (NodeSet.clear.go ns i hle).get ⟨j, h⟩ = ns.get ⟨j, h⟩ := by
+    split
+    case inl le =>
+      unfold NodeSet.clear.go
+      split
+      case inl eq =>
+        subst eq
+        exact absurd le (Nat.not_le_of_gt h)
+      case inr neq =>
+        simp
+        have hlt : i < n := Nat.lt_of_le_of_ne hle neq
+        have ih := go' (ns.unset ⟨i, hlt⟩) (i + 1) j hlt h
+        cases Nat.lt_or_ge j (i + 1) with
+        | inl lt =>
+          have eq := Nat.eq_of_ge_of_lt le lt
+          subst eq
+          simp at ih
+          exact ih
+        | inr ge =>
+          simp [ge] at ih
+          exact ih
+    case inr nle =>
+      unfold NodeSet.clear.go
+      split
+      case inl eq => rfl
+      case inr neq =>
+        simp
+        have hlt : i < n := Nat.lt_of_le_of_ne hle neq
+        have ih := go' (ns.unset ⟨i, hlt⟩) (i + 1) j hlt h
+        have : ¬ i + 1 ≤ j := by
+          intro h
+          exact absurd (Nat.le_trans (Nat.le_succ _) h) nle
+        simp [this] at ih
+        rw [ih]
+        apply NodeSet.get_unset_ne
+        simp
+        apply Nat.ne_of_gt
+        exact Nat.lt_of_not_ge nle
+termination_by go' _ => n - i
 
 open NFA
 
@@ -51,20 +225,34 @@ instance : ToString (NodeSets n) where
 def NodeSets.init (current : NodeSet n) : NodeSets n :=
   ⟨NodeSet.empty, current⟩
 
-partial def addεClosure (nfa : NFA) (i : Nat) (sets : NodeSets nfa.nodes.size) : NodeSets nfa.nodes.size :=
+-- TODO: how to avoid allocating a pair?
+-- TODO: check if the modifications don't cause copying
+def addεClosure (nfa : NFA) (i : Nat) (sets : NodeSets nfa.nodes.size) :
+  { sets' : NodeSets nfa.nodes.size // sets'.visited.count_unset ≤ sets.visited.count_unset } :=
   if hlt : i < nfa.nodes.size then
     let ⟨visited, ns⟩ := sets
-    if visited.get ⟨i, hlt⟩ then
-      sets
+    if hvis : visited.get ⟨i, hlt⟩ then
+      ⟨⟨visited, ns⟩, by simp⟩
     else
-      let visited := visited.set ⟨i, hlt⟩
+      let visited' := visited.set ⟨i, hlt⟩
+      have h : visited'.count_unset < visited.count_unset := visited.lt_count_unset hlt hvis
       let ns := ns.set ⟨i, hlt⟩
       match nfa[i] with
-      | .epsilon next => addεClosure nfa next ⟨visited, ns⟩
-      | .split next₁ next₂ => addεClosure nfa next₂ (addεClosure nfa next₁ ⟨visited, ns⟩)
-      | _ => ⟨visited, ns⟩
+      | .epsilon next =>
+        let sets' := addεClosure nfa next ⟨visited', ns⟩
+        have h' : sets'.val.visited.count_unset ≤ visited.count_unset :=
+          Nat.le_trans sets'.property (Nat.le_of_lt h)
+        ⟨sets'.val, h'⟩
+      | .split next₁ next₂ =>
+        let sets' := addεClosure nfa next₁ ⟨visited', ns⟩
+        have h' : sets'.val.visited.count_unset < visited.count_unset :=
+          Nat.lt_of_le_of_lt sets'.property h
+        let sets'' := addεClosure nfa next₂ sets'
+        ⟨sets''.val, Nat.le_trans sets''.property (Nat.le_of_lt h')⟩
+      | _ => ⟨⟨visited', ns⟩, Nat.le_of_lt h⟩
   else
-    sets
+    ⟨sets, by simp⟩
+termination_by _ => sets.visited.count_unset
 
 -- TODO: reuse allocation
 def charStep (nfa : NFA) (c : Char) (init : NodeSet nfa.nodes.size) :
@@ -84,10 +272,10 @@ where
       go nfa accum init c (i + 1) hlt
 termination_by go _ => nfa.nodes.size - i
 
-partial def NFA.NFA.run (nfa : NFA) (s : String) : Bool :=
+partial def NFA.NFA.match (nfa : NFA) (s : String) : Bool :=
   if h : 0 < nfa.nodes.size then
     let ns := addεClosure (dbgTraceVal nfa) nfa.start (NodeSets.init NodeSet.empty)
-    let ns := go nfa s 0 ns.current
+    let ns := go nfa s 0 ns.val.current
     -- This assumes that the first node is the accepting node
     ns.get ⟨0, h⟩
   else
