Regex/NFA/Tests.lean
@@ -3,17 +3,17 @@ import Regex.NFA.VM
 
 def r₁ := Regex.concat (Regex.star (Regex.char 'a')) (Regex.star (Regex.char 'b'))
 def NFA₁ := NFA.compile r₁
-#eval NFA₁.run "aaaabbbb"
-#eval NFA₁.run "ab"
-#eval NFA₁.run "c"
-#eval NFA₁.run ""
+#eval NFA₁.match "aaaabbbb"
+#eval NFA₁.match "ab"
+#eval NFA₁.match "c"
+#eval NFA₁.match ""
 
 def r₂ := Regex.star (Regex.alternate (Regex.star (Regex.char 'a')) (Regex.char 'b'))
 def NFA₂ := NFA.compile r₂
-#eval NFA₂.run "aaaabbbb"
-#eval NFA₂.run "abcab"
-#eval NFA₁.run ""
+#eval NFA₂.match "aaaabbbb"
+#eval NFA₂.match "abcab"
+#eval NFA₁.match ""
 
 def NFA₃ := NFA.compile (Regex.alternate Regex.empty (Regex.concat (Regex.char 'a') Regex.empty))
-#eval NFA₃.run ""
-#eval NFA₃.run "a"
+#eval NFA₃.match ""
+#eval NFA₃.match "a"
